move around axioms and assumptions

Cslib/Logics/Propositional/NaturalDeduction/Basic.lean
@@ -289,6 +289,83 @@ theorem DerivableIn.substAtom {Atom Atom' : Type u} [DecidableEq Atom] [Decidabl
     DerivableIn T (Γ ⊢ B) → DerivableIn (T.subst f) ((Γ.subst f) ⊢ (B >>= f))
   | ⟨D⟩ => ⟨D.substAtom f⟩
 
+/-- Move the axioms used in a derivation `D` to the context, obtaining a derivation in minimal
+logic. -/
+def Theory.Derivation.collectAxs {Γ : Ctx Atom} {B : Proposition Atom} :
+    (T.Derivation Γ B) →
+      Σ Δ : {Δ : Ctx Atom // (Δ : Theory Atom) ⊆ T}, (MPL Atom).Derivation (Γ ∪ Δ) B
+  | @ax _ _ _ _ B _ => ⟨⟨{B}, by grind⟩, ass <| by grind⟩
+  | ass _ => ⟨⟨∅, by grind⟩, ass <| by grind⟩
+  | andI D E =>
+    let ⟨Δ₁, D'⟩ := collectAxs D
+    let ⟨Δ₂, E'⟩ := collectAxs E
+    ⟨⟨Δ₁ ∪ Δ₂, by grind⟩, andI (D'.weakCtx <| by grind) (E'.weakCtx <| by grind)⟩
+  | andE₁ D => let ⟨Δ, D'⟩ := collectAxs D; ⟨Δ, andE₁ D'⟩
+  | andE₂ D => let ⟨Δ, D'⟩ := collectAxs D; ⟨Δ, andE₂ D'⟩
+  | orI₁ D => let ⟨Δ, D'⟩ := collectAxs D; ⟨Δ, orI₁ D'⟩
+  | orI₂ D => let ⟨Δ, D'⟩ := collectAxs D; ⟨Δ, orI₂ D'⟩
+  | orE D E₁ E₂ =>
+    let ⟨Δ, D'⟩ := collectAxs D
+    let ⟨Δ₁, E₁'⟩ := collectAxs E₁
+    let ⟨Δ₂, E₂'⟩ := collectAxs E₂
+    ⟨⟨Δ ∪ Δ₁ ∪ Δ₂, by grind⟩,
+      orE (D'.weakCtx <| by grind) (E₁'.weakCtx <| by grind) (E₂'.weakCtx <| by grind)⟩
+  | implI Γ D =>
+    let ⟨Δ, D'⟩ := collectAxs D; ⟨Δ, implI (Γ ∪ Δ) (D'.weakCtx <| by grind)⟩
+  | implE D E =>
+    let ⟨Δ₁, D'⟩ := collectAxs D
+    let ⟨Δ₂, E'⟩ := collectAxs E
+    ⟨⟨Δ₁ ∪ Δ₂, by grind⟩, implE (D'.weakCtx <| by grind) (E'.weakCtx <| by grind)⟩
+
+theorem DerivableIn.collectAxs {Γ : Ctx Atom} {B : Proposition Atom} :
+    DerivableIn T (Γ ⊢ B) →
+      ∃ Δ : Ctx Atom, DerivableIn (MPL Atom) ((Γ ∪ Δ) ⊢ B) ∧ ((Δ : Theory Atom) ⊆ T)
+  | ⟨D⟩ => let ⟨⟨Δ, hΔ⟩, D'⟩ := Theory.Derivation.collectAxs D; ⟨Δ, ⟨⟨D'⟩, hΔ⟩⟩
+
+/-- Remove some assumptions by moving them to the theory. -/
+def Theory.Derivation.assToAxs' {T : Theory Atom} {Γ Δ : Ctx Atom} {B : Proposition Atom} :
+    T.Derivation Γ B → (T ∪ Δ).Derivation (Γ \ Δ) B
+  | @ass _ _ _ _ B _ => by
+    by_cases B ∈ Δ
+    case pos =>
+      exact ax <| by grind
+    case neg =>
+      exact ass <| by grind
+  | ax _ => ax <| by grind
+  | andI D E => andI (assToAxs' D) (assToAxs' E)
+  | andE₁ D => andE₁ (assToAxs' D)
+  | andE₂ D => andE₂ (assToAxs' D)
+  | orI₁ D => orI₁ (assToAxs' D)
+  | orI₂ D => orI₂ (assToAxs' D)
+  | @orE _ _ _ _ A' B C D E₁ E₂ =>
+    orE (assToAxs' D)
+      ((assToAxs' (Δ := Δ) (B := C) E₁).weakCtx <| by grind)
+      ((assToAxs' (Δ := Δ) (B := C) E₂).weakCtx <| by grind)
+  | @implI _ _ _ A' B _ D =>
+    implI _ ((assToAxs' (Δ := Δ) (B := B) D).weakCtx <| by grind)
+  | implE D E => implE (assToAxs' D) (assToAxs' E)
+
+/-- Remove dependence on some assumptions by adding them to the theory. -/
+def Theory.Derivation.assToAxs {T : Theory Atom} {Γ Δ : Ctx Atom} {B : Proposition Atom}
+    (D : T.Derivation (Γ ∪ Δ) B) : (T ∪ Δ).Derivation Γ B := (assToAxs' D).weakCtx <| by grind
+
+theorem DerivableIn.ass_to_axs {T : Theory Atom} {Γ Δ : Ctx Atom} {B : Proposition Atom} :
+    DerivableIn T ((Γ ∪ Δ) ⊢ B) → DerivableIn (T ∪ Δ : Theory Atom) (Γ ⊢ B)
+  | ⟨D⟩ => ⟨Theory.Derivation.assToAxs D⟩
+
+def Theory.Derivation.axsToAss {T : Theory Atom} {Γ Δ : Ctx Atom} {B : Proposition Atom}
+    (D : (T ∪ Δ : Theory Atom)⇓(Γ ⊢ B)) : T⇓((Γ ∪ Δ) ⊢ B) :=
+  let ⟨⟨Δ', hΔ'⟩, D'⟩ := collectAxs D
+  (D'.assToAxs' (Δ := Δ' \ Δ)).weak (by grind) (by grind)
+
+theorem DerivableIn.axs_to_ass {T : Theory Atom} {Γ Δ : Ctx Atom} {B : Proposition Atom} :
+    DerivableIn (T ∪ Δ : Theory Atom) (Γ ⊢ B) → DerivableIn T ((Γ ∪ Δ) ⊢ B)
+  | ⟨D⟩ => ⟨D.axsToAss⟩
+
+theorem DerivableIn.iff_derivableIn_extension {Γ Δ : Ctx Atom} {B : Proposition Atom} :
+    DerivableIn T ((Γ ∪ Δ) ⊢ B) ↔ DerivableIn (T ∪ Δ : Theory Atom) (Γ ⊢ B) :=
+  ⟨DerivableIn.ass_to_axs, DerivableIn.axs_to_ass⟩
+
 /-! ### Properties of equivalence -/
 
 /-- A derivation of the canonical tautology. -/
